grammatik/Grammatik/Kette108.lean
@@ -303,7 +303,7 @@ theorem kette_108_nebenlaeufig :
     Laufzeit E8 (speicherR E8.sp0) (initRuhe E8.starts) ∧
     Ziel E8.P.mitRuhe E8.S.mitRuhe O8.mitRuhe 0 (RufStartG E8.P.mitRuhe (speicherR E8.sp0)
       (initRuhe E8.starts)) (RufStartG E8.P.mitRuhe (speicherR E8.sp0) (initRuhe E8.starts)) := by
-  have hL := laufzeit_initRuhe E8 (by decide)
+  have hL := laufzeit_initRuhe E8
   exact ⟨hL, (schlusssatz kette_108 O8 hw8 tvOrc tvXR tvXR_funktional
     (fun f => CallAt EL8.lay tvOrc tvXR (kProg zert108) 1 (fnNr f)) (fun _ => 1)
     (fun _ _ _ _ _ h => h) (speicherR E8.sp0) init8 start8).2.2.2.2.2.2.2.2.1.2.2 0 _ _ hL _ .start⟩
